The sum of a [[Sequences]] of terms.

### Sigma notation
Given a function $f$ and two integers $A$ and $B$ (with $A \leq B$), we write
$$\sum_{n=A}^{B} f(n) = f(A) + f(A + 1) + \ldots + f(B)$$

i.e., adding up the results when $f$ is applied to each of the integers from $A$ to $B$.

$A$ is the starting point, the function is $f(n)$, and $B$ is the end point.
### Sigma Notation Laws:
*Note*: There's not necessarily a unique way of writing a sum using Sigma Notation. 

### Linearity of sigma notation

If $c$ is any constant (i.e., does not depend on $n$), then
$$
\sum_{i=1}^{n} c = nc
$$
and
$$
\sum_{i=1}^{n} c a_i = c \sum_{i=1}^{n} a_i
$$
and
$$
\sum_{i=1}^{n} (a_i + b_i)
$$
##### Splitting a Sum in Sigma Notation
If $m, n$ are integers with $1 < m < n$, then
$$
\sum_{i=1}^{n} a_i = \sum_{i=1}^{m} a_i + \sum_{i=m+1}^{n} a_i.
$$
##### Sums of Powers (Used a lot - memorise them):
The sum of the first $n$ integers is given by:

$$
\sum_{i=1}^{n} 1 = n
$$

The sum of the first $n$ natural numbers is:

$$
\sum_{i=1}^{n} i = \frac{1}{2}n(n + 1) = \frac{n^2}{2} + \frac{n}{2}
$$


The sum of the squares of the first $n$ natural numbers is:

$$
\sum_{i=1}^{n} i^2 = \frac{1}{6}n(n + 1)(2n + 1) = \frac{n^3}{3} + \frac{n^2}{2} + \frac{n}{6}
$$


The sum of the cubes of the first $n$ natural numbers is:

$$
\sum_{i=1}^{n} i^3 = \frac{1}{4}n^2(n + 1)^2 = \frac{n^4}{4} + \frac{n^3}{2} + \frac{n^2}{4}
$$

